a function that writes a ref checks with native tactic and extracts too

examples/dsls/mini_steel/_output/Refl_Typing_Builtins.ml
@@ -1,0 +1,30 @@
+open FStar_Syntax_Syntax
+open FStar_Reflection_Types
+
+let dummy_range = FStar_Compiler_Range.dummyRange
+let underscore = FStar_Ident.mk_ident ("_", dummy_range)
+let int_as_bv (n:Prims.int) = { ppname = underscore; index = n; sort = tun}
+
+let open_term (t:term) (v:Prims.int)
+  : term
+  = let subst = DB (Z.zero, int_as_bv v) in
+    FStar_Syntax_Subst.subst [subst] t
+
+let close_term (t:term) (v:Prims.int)
+  : term
+  = let subst = NM (int_as_bv v, Z.zero) in
+    FStar_Syntax_Subst.subst [subst] t
+
+let open_with (t:term) (v:term)
+  : term
+  = let neg = int_as_bv (Z.of_int (-1)) in (* a temporary non-clashing name *)
+    let opened_t = FStar_Syntax_Subst.subst [DB(Z.zero, neg)] t in
+    (* gets substituted away immediately *)
+    FStar_Syntax_Subst.subst [NT(neg, v)] opened_t
+
+let rename (t:term) (x:Prims.int) (y:Prims.int)
+  : term
+  = FStar_Syntax_Subst.subst [NT(int_as_bv x, bv_to_name (int_as_bv y))] t
+
+
+  
